update San to satisfies start_pc_ok

compiler/backend/San/SanScript.sml
@@ -12,7 +12,7 @@ val san_prog_asm_def = Define`
     T, (Inst (Mem Load 6 (Addr 5 20000w)));
     F, (Inst (Arith (Binop Add 7 6 (Imm 1w))));
     T, (Inst (Mem Store 7 (Addr 5 20008w)));
-    F, (JumpReg 5)]`; (* jump to the halt pc *)
+    F, (Jump 16w)]`; (* jump to the halt pc *)
 
 val asm2ast_def = Define`
   asm2ast = MAP (\(b,asm). (b,riscv_ast asm))`;
@@ -75,9 +75,10 @@ val san_end_pcs_simp = EVAL ``san_end_ffi_pcs``;
 
 val san_config_def = Define`
   san_config =
-  <| prog_addresses := {x | x < 1000w} DELETE 0w DELETE n2w ffi_offset DIFF
-  flip MEM san_ffi_pcs
-   ; shared_addresses := {20000w;20008w}
+  <| prog_addresses := {x | x < 1000w} DELETE 0w DELETE n2w ffi_offset
+    DIFF {a| a >= EL 0 ffi_entry_pcs /\ a < EL 0 san_end_ffi_pcs}
+    DIFF {a| a >= EL 1 ffi_entry_pcs /\ a < EL 1 san_end_ffi_pcs}
+   ; shared_addresses := {a| a >= 20000w /\ a < 20016w}
    ; ffi_entry_pcs := san_ffi_pcs
    ; ffi_names := ["MappedRead";"MappedWrite"]
    ; ptr_reg := ARB
@@ -87,8 +88,8 @@ val san_config_def = Define`
    ; ffi_interfer := san_ffi_interfer
     (san_mmio_info: num -> word8 # word64 # num # word64)
    ; next_interfer := K I
-   ; halt_pc := 0w
-   ; ccache_pc := n2w ffi_offset
+   ; halt_pc := n2w ffi_offset
+   ; ccache_pc := 0w
    ; ccache_interfer :=ARB
    ; target := riscv_target
    ; mmio_info := san_mmio_info|>`;
@@ -138,7 +139,7 @@ val riscv_inst_defs = map (fst o snd) $
   filter (fn n => snd (snd n) = Def) $ DB.match ["riscv"] ``_``;
 
 val _ = computeLib.add_funs
-  [Encode_def,Itype_def,Stype_def,opc_def,word_concat_def];
+  [Encode_def,Itype_def,Stype_def,UJtype,opc_def,word_concat_def];
 
 val san_program_simp = EVAL ``san_program``;
 
@@ -163,8 +164,6 @@ val decode_conv =
   EVAL THENC
   SIMP_CONV (srw_ss()) [v2w_def] THENC
   EVAL;
-
-val san_decode_inst_1 = decode_conv ``Decode 25235w``;
 
 fun pattern_conv pat conv_f = DEPTH_CONV
   (fn tm =>
@@ -197,79 +196,27 @@ val san_prog_addr_simp =
 
 val san_mmio_info_simp = EVAL ``san_mmio_info``;
 
-Theorem valid_mapped_read_simp:
-   is_valid_mapped_read 36w 8w 20000w 6 40w
-     <|config := riscv_config; next := riscv_next;
-       get_pc := (λs. s.c_PC s.procID);
-       get_reg := (λs. s.c_gpr s.procID ∘ n2w);
-       get_byte := riscv_state_MEM8; state_ok := riscv_ok;
-       proj := riscv_proj|>
-     <|MEM8 :=
-         word_EL
-           [0w; 0w; 0w; 0w; 0w; 0w; 0w; 0w; 0w; 0w; 0w; 0w;
-            0w; 0w; 0w; 0w; 0w; 0w; 0w; 0w; 0w; 0w; 0w; 0w;
-            0w; 0w; 0w; 0w; 0w; 0w; 0w; 0w; 147w; 98w; 0w;
-            0w; 3w; 179w; 2w; 226w; 147w; 3w; 19w; 0w; 35w;
-            180w; 114w; 226w; 103w; 128w; 2w; 0w] 0w;
-       c_MCSR :=
-         ARB⦇
-           0w ↦
-             <|mcpuid := <|ArchBase := 2w|>;
-               mstatus := <|VM := 0w|> |>
-         ⦈; c_NextFetch := ARB⦇0w ↦ NONE⦈;
-       c_PC := (K 0w)⦇0w ↦ 36w⦈;
-       c_Skip := ARB.c_Skip⦇0w ↦ 4w⦈;
-       c_gpr := ARB.c_gpr⦇0w ↦ (ARB.c_gpr 0w)⦇5w ↦ 0w⦈⦈;
-       exception := NoException; procID := 0w|>
-Proof
-  simp[is_valid_mapped_read_def] \\
-  qexistsl [`5`, `20000w`] \\
-  simp[riscv_config_def, riscv_enc_def,riscv_ast_def,LIST_BIND_def] \\
-  EVAL_TAC
-QED
+fun valid_mapped_read_tac reg address =
+  qpat_abbrev_tac `_r = is_valid_mapped_read _` \\
+  `_r` by (
+    qunabbrev_tac `_r` \\
+    simp[is_valid_mapped_read_def] \\
+    qexistsl [reg, address] \\
+    simp[riscv_config_def, riscv_enc_def,riscv_ast_def,LIST_BIND_def] \\
+    EVAL_TAC
+  ) \\
+  qunabbrev_tac `_r`;
 
-Theorem valid_mapped_write_simp:
-  is_valid_mapped_write 44w 8w 20008w 7 48w
-     <|config := riscv_config; next := riscv_next;
-       get_pc := (λs. s.c_PC s.procID);
-       get_reg := (λs. s.c_gpr s.procID ∘ n2w);
-       get_byte := riscv_state_MEM8; state_ok := riscv_ok;
-       proj := riscv_proj|>
-     <|MEM8 :=
-         word_EL
-           [0w; 0w; 0w; 0w; 0w; 0w; 0w; 0w; 0w; 0w; 0w; 0w;
-            0w; 0w; 0w; 0w; 0w; 0w; 0w; 0w; 0w; 0w; 0w; 0w;
-            0w; 0w; 0w; 0w; 0w; 0w; 0w; 0w; 147w; 98w; 0w;
-            0w; 3w; 179w; 2w; 226w; 147w; 3w; 19w; 0w; 35w;
-            180w; 114w; 226w; 103w; 128w; 2w; 0w] 0w;
-       c_MCSR :=
-         ARB⦇
-           0w ↦
-             <|mcpuid := <|ArchBase := 2w|>;
-               mstatus := <|VM := 0w|> |>
-         ⦈; c_NextFetch := ARB⦇0w ↦ NONE⦈;
-       c_PC := (K 0w)⦇0w ↦ 44w⦈;
-       c_Skip := ARB.c_Skip⦇0w ↦ 4w⦈;
-       c_gpr :=
-         (λpid r.
-              if pid = 0w ∧ r = 6w then 20w
-              else
-                (if pid = 0w then (ARB.c_gpr 0w)⦇5w ↦ 0w⦈
-                 else ARB.c_gpr pid) r)⦇
-           0w ↦
-             (λr.
-                  if r = 6w then 20w
-                  else if r = 5w then 0w
-                  else ARB.c_gpr 0w r)⦇
-               7w ↦ 21w
-             ⦈
-         ⦈; exception := NoException; procID := 0w|>
-Proof
-  simp[is_valid_mapped_write_def] \\
-  qexistsl [`5`, `20008w`] \\
-  simp[riscv_config_def, riscv_enc_def,riscv_ast_def,LIST_BIND_def] \\
-  EVAL_TAC
-QED
+fun valid_mapped_write_tac reg address =
+ qpat_abbrev_tac `_w = is_valid_mapped_read _` \\
+  `_w` by (
+    qunabbrev_tac `_w` \\
+    simp[is_valid_mapped_write_def] \\
+    qexistsl [reg, address] \\
+    simp[riscv_config_def, riscv_enc_def,riscv_ast_def,LIST_BIND_def] \\
+    EVAL_TAC
+  ) \\
+  qunabbrev_tac `_w`;
 
 Theorem san_io_event_length:
   LENGTH (SND(SND(san_result 10))).io_events = 2
@@ -287,7 +234,7 @@ Proof
   simp[Once evaluate_def,APPLY_UPDATE_THM] \\
   simp[find_index_def, san_ffi_pcs_simp] \\
   simp[san_mmio_info_simp,APPLY_UPDATE_THM] \\
-  simp[valid_mapped_read_simp] \\
+  valid_mapped_read_tac `5` `20000w` \\
   simp[call_FFI_def,san_init_ffi_state_def,san_oracle_def] \\
   simp[length_pad_right,
     EVAL ``LENGTH (addr2w8list (20000w:word64))``] \\
@@ -300,7 +247,7 @@ Proof
   simp[Once evaluate_def,APPLY_UPDATE_THM] \\
   simp[find_index_def,san_ffi_pcs_simp] \\
   simp[san_mmio_info_simp,APPLY_UPDATE_THM] \\
-  simp[valid_mapped_write_simp] \\
+  valid_mapped_write_tac `5` `20008w` \\
   simp[call_FFI_def,san_init_ffi_state_def,san_oracle_def] \\
   simp[length_pad_right,
     EVAL ``LENGTH (addr2w8list 20008w)``,
@@ -312,6 +259,27 @@ Proof
   next_state_tac \\
   riscv_ok_tac \\
   simp[Once evaluate_def, APPLY_UPDATE_THM]
+QED
+
+Theorem san_start_pc_ok:
+  start_pc_ok san_config 32w
+Proof
+  rw[start_pc_ok_def] \\
+  fs[san_config_def, EVAL ``ffi_offset``] \\
+  qexists `0` \\
+  rw[san_ffi_pcs_def,san_ffi_pcs_simp,san_mmio_info_def,
+    san_prog_addr_simp,DISJOINT_DEF] \\
+  >- (
+    fs[mmio_pcs_min_index_def] \\
+    irule some_intro \\
+    rw[] \\
+
+  )
+QED
+
+Theorem san_ffi_interfer_ok:
+  ffi_interfer_ok 
+Proof
 QED
 
 val () = export_theory();
